{
 "cells": [
  {
   "cell_type": "markdown",
   "metadata": {},
   "source": [
    "Discrete Lecture 1 Assignments\n",
    "=="
   ]
  },
  {
   "cell_type": "markdown",
   "metadata": {},
   "source": [
    " NAME: CARLOS MIGUEL K. JAKOSALEM <br>\n",
    " BSCS - 1"
   ]
  },
  {
   "cell_type": "markdown",
   "metadata": {},
   "source": [
    "*1. Recall the definition of a rational number, denoted as $\\mathbb{Q}$. Prove that Euler's number $e = \\sum_{k=0}^\\infty \\frac{1}{k!} \\notin \\mathbb{Q}$. A factorial is defined as $k! = (k)(k-1)(k-2)(k-3)..., \\forall k \\in \\mathbb{Z}^+$, note that $0! = 1$. Furthermore, a sum notation $\\sum_{k=0}^\\infty k = 0+ 1 + 2 + 3 +....+...$.*\n",
    "\n",
    "\n",
    "Step 1:\n",
    "\n",
    "Use proof by contradiction in order to show that Euler's constant $e$ is irrational\n",
    "\n",
    "Assuming $e$ is rational, we can represent it as the fraction of two integers $p$ and $q$, where $q \\neq 0$. Hence, $e = \\frac{p}{q}$.\n",
    "\n",
    "Step 2:\n",
    "\n",
    "Recall $e$ as the infinite series $\\sum_{k=0}^\\infty \\frac{1}{k!}$. Meaning:\n",
    "\n",
    "$ e = \\frac{1}{0!} + \\frac{1}{1!} + \\frac{1}{2!} + \\frac{1}{3!} + \\ldots $\n",
    "\n",
    "Step 3:\n",
    "\n",
    "Considering the partial sum of the series:\n",
    "\n",
    "$ S_n = \\frac{1}{0!} + \\frac{1}{1!} + \\frac{1}{2!} + \\frac{1}{3!} + \\ldots + \\frac{1}{n!} $\n",
    "\n",
    "for positive integer $n$. Since each term is positive, $S_n$ increases, converging to $e$ as $n$ approaches infinity.\n",
    "\n",
    "Step 4:\n",
    "\n",
    "Using this expression:\n",
    "\n",
    "$ q! \\cdot S_n = q! \\cdot \\left(\\frac{1}{0!} + \\frac{1}{1!} + \\frac{1}{2!} + \\frac{1}{3!} + \\ldots + \\frac{1}{n!}\\right) $\n",
    "\n",
    "Step 5:\n",
    "\n",
    "Expounding on the expression:\n",
    "\n",
    "$ q! \\cdot S_n = q! + \\frac{q!}{1!} + \\frac{q!}{2!} + \\frac{q!}{3!} + \\ldots + \\frac{q!}{n!} $\n",
    "\n",
    "Step 6:\n",
    "\n",
    "All of the terms in the expression are integers. Since $S_n$ intersects to $e$, $q! \\cdot S_n$ should be close to $q! \\cdot e = p$. Implying that $p - q! \\cdot S_n$ is a small integer.\n",
    "\n",
    "$ p - q! \\cdot S_n = p - (q! + \\frac{q!}{1!} + \\frac{q!}{2!} + \\frac{q!}{3!} + \\ldots + \\frac{q!}{n!}) $\n",
    "\n",
    "$ p - q! \\cdot S_n = p - q! - \\frac{q!}{1!} - \\frac{q!}{2!} - \\frac{q!}{3!} - \\ldots - \\frac{q!}{n!} $\n",
    "\n",
    "$ p - q! \\cdot S_n = (p - q!) - \\frac{q!}{1!} - \\frac{q!}{2!} - \\frac{q!}{3!} - \\ldots - \\frac{q!}{n!} $\n",
    "\n",
    "Step 7:\n",
    "\n",
    "The terms in the parentheses are all integers, and the summation in each term is a fraction with a denominator greater than 1. Thus, $p - q! \\cdot S_n$ is a non-zero positive integer.\n",
    "\n",
    "However, this contradicts that $e = \\frac{p}{q}$ because $q! \\cdot S_n$ should be close to $p$ but is not equal, leading to a contradiction.\n",
    "\n",
    "Therefore, $e$ being rational is not correct and is actually irrational.\n",
    "\n",
    "****"
   ]
  },
  {
   "cell_type": "markdown",
   "metadata": {},
   "source": [
    "2. Prove Minkowski's Inequality for sums, $\\forall \\ p>1, (a_k, b_k)>0$:\n",
    "\n",
    "\\begin{gather}\n",
    "\\begin{bmatrix}\n",
    "\\sum_{k=1}^n |a_k + b_k|^p\n",
    "\\end{bmatrix}^\\frac{1}{p}\n",
    "\\leq\n",
    "\\begin{bmatrix}\n",
    "\\sum_{k=1}^n |a_k|^p\n",
    "\\end{bmatrix}^\\frac{1}{p}\n",
    "+\n",
    "\\begin{bmatrix}\n",
    "\\sum_{k=1}^n |b_k|^p\n",
    "\\end{bmatrix}^\\frac{1}{p}\n",
    "\\end{gather}\n",
    "\n",
    "\n",
    "Step 1:\n",
    "To prove Minkowski's inequality for sums, we will make use Hölder's inequality. Hölder's inequality explains that for any two sequences of real numbers $(x_k)$ and $(y_k)$ and any $p>1$ such that $\\frac{1}{p} + \\frac{1}{q} = 1$, the following holds:\n",
    "\n",
    "$\\sum_{k=1}^n |x_k y_k| \\leq \\left( \\sum_{k=1}^n |x_k|^p \\right)^{\\frac{1}{p}} \\left( \\sum_{k=1}^n |y_k|^q \\right)^{\\frac{1}{q}}$\n",
    "\n",
    "Step 2:\n",
    "Now, let's define $x_k = \\frac{|a_k|^p}{\\left(\\sum_{k=1}^n |a_k|^p\\right)^{\\frac{1}{p}}}$ and $y_k = \\frac{|b_k|^p}{\\left(\\sum_{k=1}^n |b_k|^p\\right)^{\\frac{1}{p}}}$. \n",
    "\n",
    "Step 3:\n",
    "Then, we have:\n",
    "\n",
    "\\begin{align*}\n",
    "\\sum_{k=1}^n |a_k + b_k|^p &= \\sum_{k=1}^n |a_k + b_k|^p \\cdot 1^{1-p} \\\\\n",
    "&\\leq \\left( \\sum_{k=1}^n |a_k|^p \\right)^{\\frac{1}{p}} \\left( \\sum_{k=1}^n |b_k|^p \\right)^{\\frac{1}{q}} \\left( \\sum_{k=1}^n 1^{q} \\right)^{1/q} \\\\\n",
    "&= \\left( \\sum_{k=1}^n |a_k|^p \\right)^{\\frac{1}{p}} \\left( \\sum_{k=1}^n |b_k|^p \\right)^{\\frac{1}{p}} \\left( \\sum_{k=1}^n 1 \\right)^{1/q} \\\\\n",
    "&= \\left( \\sum_{k=1}^n |a_k|^p \\right)^{\\frac{1}{p}} \\left( \\sum_{k=1}^n |b_k|^p \\right)^{\\frac{1}{p}} n^{1/q}\n",
    "\\end{align*}\n",
    "\n",
    "Given $\\frac{1}{p} + \\frac{1}{q} = 1$, we find $q = \\frac{p}{p-1}$.\n",
    "\n",
    "So, $n^{1/q} = n^{\\frac{p-1}{p}} = n^{\\frac{1}{p-1}}$.\n",
    "\n",
    "Giving us:\n",
    "\n",
    "$\\sum_{k=1}^n |a_k + b_k|^p \\leq \\left( \\sum_{k=1}^n |a_k|^p \\right)^{\\frac{1}{p}} \\left( \\sum_{k=1}^n |b_k|^p \\right)^{\\frac{1}{p}} n^{\\frac{1}{p-1}}$\n",
    "\n",
    "Step 4:\n",
    "Divide both sides by $n^{\\frac{1}{p-1}}$:\n",
    "\n",
    "$\\frac{1}{n^{\\frac{1}{p-1}}} \\sum_{k=1}^n |a_k + b_k|^p \\leq \\left( \\sum_{k=1}^n |a_k|^p \\right)^{\\frac{1}{p}} \\left( \\sum_{k=1}^n |b_k|^p \\right)^{\\frac{1}{p}}$\n",
    "\n",
    "Step 5:\n",
    "Take $p$-th root on each sides:\n",
    "\n",
    "$\\left( \\frac{1}{n} \\sum_{k=1}^n |a_k + b_k|^p \\right)^{\\frac{1}{p}} \\leq \\left( \\sum_{k=1}^n |a_k|^p \\right)^{\\frac{1}{p}} \\left( \\sum_{k=1}^n |b_k|^p \\right)^{\\frac{1}{p}}$\n",
    "\n",
    "With this Minkowski's inequality for sums is proved.\n",
    "\n",
    "****\n"
   ]
  },
  {
   "cell_type": "markdown",
   "metadata": {},
   "source": [
    "*3. Prove the triangle inequality $|x+y| \\leq |x| + |y|, \\forall (x,y) \\in \\mathbb{R}$*\n",
    "\n",
    "\n",
    "Step 1:\n",
    "\n",
    "To prove triangle inequality $|x+y| \\leq |x| + |y|$, we have to consider the cases where $x$ and $y$ are both positive, negative, or of different signs.\n",
    "\n",
    "Step 2:\n",
    "\n",
    "Case 1: $x$ and $y$ are both positive:\n",
    "$|x+y| = x+y$ \n",
    "$|x| + |y| = x + y$ \n",
    "Since $x$ and $y$ are both positive, their absolute values are equal to the original values. So $|x+y| = |x| + |y|$ is true.\n",
    "\n",
    "Step 3:\n",
    "\n",
    "Case 2: $x$ and $y$ are both negative:\n",
    "$|x+y| = -(x+y) = -x - y$ \n",
    "$|x| + |y| = -x - y$ \n",
    "Since $x$ and $y$ are both negative, their absolute values are negations of their original values. So $|x+y| = |x| + |y|$ is true.\n",
    "\n",
    "Step 4:\n",
    "\n",
    "Case 3: $x$ and $y$ have different signs:\n",
    "Assume $x > 0$ and $y < 0$. Then,\n",
    "$|x+y| = |x-y|$ \n",
    "$|x| + |y| = x + (-y) = x - y$ \n",
    "Since $x > y$ , $|x-y| = x-y$, so $|x+y| = |x| + |y|$ is true.\n",
    "\n",
    "Step 5:\n",
    "\n",
    "In all cases, we have shown that $|x+y| \\leq |x| + |y|$, proving the triangle inequality for $x$ and $y$.\n",
    "\n",
    "****"
   ]
  },
  {
   "cell_type": "markdown",
   "metadata": {},
   "source": [
    "4. Prove Sedrakayan's Lemma $\\forall u_i, v_i \\in \\mathbb{R}^+$:\n",
    "\n",
    "\\begin{gather}\n",
    "\\frac{(\\sum_{i=1}^n u_i)^2}{\\sum_{i=1}^n v_i}\n",
    "\\leq\n",
    "\\sum_{i=1}^n \\frac{(u_i)^2}{v_i}\n",
    "\\end{gather}\n",
    "\n",
    "ANSWER:\n",
    "-\n",
    "\n",
    "Step 1:\n",
    "\n",
    "Sedrakayan's Lemma states that:\n",
    "\n",
    "For any positive real numbers $u_i$ and $v_i$ (where $i$ ranges from 1 to $n$):\n",
    "\n",
    "$\\frac{(\\sum_{i=1}^n u_i)^2}{\\sum_{i=1}^n v_i} \\leq \\sum_{i=1}^n \\frac{u_i^2}{v_i}$\n",
    "\n",
    "To prove this, we will make use of the Cauchy-Schwarz Inequality.\n",
    "\n",
    "Step 2:\n",
    "\n",
    "1. Define two vectors:\n",
    "   - $\\mathbf{u} = (u_1, u_2, ..., u_n)$\n",
    "   - $\\mathbf{v} = (\\sqrt{v_1}, \\sqrt{v_2}, ..., \\sqrt{v_n})$\n",
    "\n",
    "Step 3:\n",
    "\n",
    "2. Apply the Cauchy-Schwarz Inequality for the products of the vectors. This inequality states that the square of the dot product of two vectors is less than or equal to the product of the squares of their magnitudes.\n",
    "\n",
    "Step 4:\n",
    "\n",
    "For the sum of $u_i$, we have:\n",
    "$(\\sum_{i=1}^n u_i)^2 \\leq n (\\sum_{i=1}^n u_i^2)$\n",
    "\n",
    "For the sum of $\\sqrt{v_i}$, we have:\n",
    "$(\\sum_{i=1}^n \\sqrt{v_i})^2 \\leq n (\\sum_{i=1}^n v_i)$\n",
    "\n",
    "Step 5:\n",
    "\n",
    "3. Rearrange:\n",
    "$\\frac{(\\sum_{i=1}^n u_i)^2}{\\sum_{i=1}^n v_i} \\leq \\frac{\\sum_{i=1}^n u_i^2}{n}$\n",
    "\n",
    "Step 6:\n",
    "\n",
    "Knowing: $\\mathbf{u} \\cdot \\mathbf{v} \\leq |\\mathbf{u}| \\cdot |\\mathbf{v}|$. Expand the dot product:\n",
    "$\\sum_{i=1}^n u_i \\sqrt{v_i} \\leq \\sqrt{\\sum_{i=1}^n u_i^2} \\sqrt{\\sum_{i=1}^n v_i}$\n",
    "\n",
    "Step 7:\n",
    "\n",
    "Square each side:\n",
    "$(\\sum_{i=1}^n u_i \\sqrt{v_i})^2 \\leq (\\sum_{i=1}^n u_i^2)(\\sum_{i=1}^n v_i)$\n",
    "\n",
    "Step 8:\n",
    "\n",
    "Substitute $\\mathbf{u} = (u_1, u_2, ..., u_n)$ and $\\mathbf{v} = (\\sqrt{v_1}, \\sqrt{v_2}, ..., \\sqrt{v_n})$:\n",
    "$\\left(\\sum_{i=1}^n u_i \\sqrt{v_i}\\right)^2 \\leq \\left(\\sum_{i=1}^n u_i^2\\right) \\left(\\sum_{i=1}^n v_i\\right)$\n",
    "\n",
    "Step 9:\n",
    "\n",
    "Rearrange:\n",
    "$\\frac{(\\sum_{i=1}^n u_i)^2}{\\sum_{i=1}^n v_i} \\leq \\sum_{i=1}^n \\frac{u_i^2}{v_i}$\n",
    "\n",
    "Proving Sedrakayan's Lemma."
   ]
  },
  {
   "cell_type": "markdown",
   "metadata": {},
   "source": [
    "Extra Problems\n",
    "="
   ]
  },
  {
   "cell_type": "markdown",
   "metadata": {},
   "source": [
    "1. Consider the functions $f(x) = 2x+1$, $g(x)=2y-1$, $j(x) = |f(x)+g(x)|$, and $h(x) = j(x)^2$, show for the following inequality that:\n",
    "\\begin{gathered}\n",
    "\\sqrt{|f(x)|^2} \\geq \\sqrt{h(x)} - \\sqrt{|g(x)|^2}, \\forall (x,y) \\in \\mathbb{Z}^+\n",
    "\\end{gathered}"
   ]
  },
  {
   "cell_type": "markdown",
   "metadata": {},
   "source": [
    "Step 1: Substitute\n",
    "\n",
    "\\begin{gathered}\n",
    "\\sqrt{\\left|f\\left(x\\right)\\right|^2}\\ge \\sqrt{\\left|f\\left(x\\right)+g\\left(x\\right)\\right|^2}-\\sqrt{\\left|g\\left(x\\right)\\right|^2}\n",
    "\\end{gathered}\n",
    "\n",
    "Step 2: Using of Minkowski's Inequality for sums\n",
    "\n",
    "\\begin{gathered}\n",
    "\\left|f\\left(x\\right)\\right|\\ge \\left|f\\left(x\\right)+g\\left(x\\right)\\right|-\\left|g\\left(x\\right)\\right|\n",
    "\\end{gathered}\n",
    "\n",
    "Step 3: Transpose\n",
    "\n",
    "\\begin{gathered}\n",
    "\\left|f\\left(x\\right)\\right|+\\left|g\\left(x\\right)\\right|\\ge \\left|f\\left(x\\right)+g\\left(x\\right)\\right|\n",
    "\\end{gathered}\n",
    "\n",
    "Step 4: Rearrange to get Triangle Inequality\n",
    "\n",
    "\\begin{gathered}\n",
    "\\left|f\\left(x\\right)+g\\left(x\\right)\\right|\\le \\left|f\\left(x\\right)\\right|+\\left|g\\left(x\\right)\\right|\n",
    "\\end{gathered}\n",
    "\n",
    "Step 5: Prove with the case: $f\\left(x\\right)>0$, and $g\\left(x\\right)>0$, Since $\\forall (x,y) \\in \\mathbb{Z}^+$\n",
    "\n",
    " Let $\\left|f\\left(x\\right)+g\\left(x\\right)\\right|=f\\left(x\\right)+g\\left(x\\right)$, and $|x|=x$, $|y|=y$\n",
    "\n",
    "Step 6: Substitute:\n",
    "\\begin{gathered}\n",
    "\\left|f\\left(x\\right)+g\\left(x\\right)\\right|=f\\left(x\\right)+g\\left(x\\right)=\\left|f\\left(x\\right)\\right|+\\left|g\\left(x\\right)\\right|\n",
    "\\end{gathered}\n",
    "\n"
   ]
  },
  {
   "cell_type": "markdown",
   "metadata": {},
   "source": [
    "2. Prove Sedrakayan's Lemma if $u_i, v_i$ are square roots of an even integers:\n",
    "\\begin{gathered}\n",
    "\\frac{(\\Sigma_{i=1}^n u_i)^2}{\\Sigma_{i=1}^n v_i}\n",
    "\\leq\n",
    "\\Sigma_{i=1}^n \\frac{(u_i)^2}{v_i}\n",
    "\\end{gathered}"
   ]
  },
  {
   "cell_type": "markdown",
   "metadata": {},
   "source": [
    "Let $ u_i = \\sqrt{2a_i} $ and $ v_i = \\sqrt{2b_i} $, where $ a_i $ and $ b_i $ are positive integers.\n",
    "\n",
    "$$ \\frac{\\left( \\sum_{i=1}^n \\sqrt{2a_i} \\right)^2}{\\sum_{i=1}^n \\sqrt{2b_i}} \\leq \\sum_{i=1}^n \\frac{(2a_i)}{(2b_i)}$$\n",
    "\n",
    "Step 1: Expand the terms\n",
    "\n",
    "$$\\frac{\\left( \\sum_{i=1}^n \\sqrt{2a_i} \\right)^2}{\\sum_{i=1}^n \\sqrt{2b_i}} = \\frac{\\left( \\sum_{i=1}^n \\sqrt{2a_i} \\right) \\left( \\sum_{i=1}^n \\sqrt{2a_i} \\right)}{\\sum_{i=1}^n \\sqrt{2b_i}}\n",
    ", \\quad\n",
    "\\sum_{i=1}^n \\frac{(2a_i)}{(2b_i)} = \\sum_{i=1}^n \\frac{2a_i}{2b_i}$$\n",
    "\n",
    "\n",
    "Step 2: Rewrite\n",
    "\n",
    "\n",
    "$$\\frac{\\left( \\sum_{i=1}^n \\sqrt{2a_i} \\right)^2}{\\sum_{i=1}^n \\sqrt{2b_i}} \\leq \\sum_{i=1}^n \\frac{\\sqrt{2a_i}^2}{\\sqrt{2b_i}}$$\n",
    "\n",
    "Step 3: Consider the identity:\n",
    "\n",
    "$$\\left( \\sum_{i=1}^n x_i \\right)^2 = \\sum_{i=1}^n x_i^2 + 2 \\sum_{1 \\leq i < j \\leq n} x_i x_j$$\n",
    "\n",
    "Step 4: Apply the identity\n",
    "\n",
    "$$\\frac{\\left( \\sum_{i=1}^n \\sqrt{2a_i} \\right)^2}{\\sum_{i=1}^n \\sqrt{2b_i}} = \\frac{\\sum_{i=1}^n (2a_i) + 2 \\sum_{1 \\leq i < j \\leq n} \\sqrt{2a_i} \\sqrt{2a_j}}{\\sum_{i=1}^n \\sqrt{2b_i}}$$\n",
    "\n",
    "Step 5:\n",
    "\n",
    " $2a_i$ and $2b_i$ and $2 \\sum_{1 \\leq i < j \\leq n} \\sqrt{2a_i} \\sqrt{2a_j}$ are even integers.\n",
    "\n",
    "$$\\frac{\\sum_{i=1}^n (2a_i)}{\\sum_{i=1}^n \\sqrt{2b_i}} + \\frac{2 \\sum_{1 \\leq i < j \\leq n} \\sqrt{2a_i} \\sqrt{2a_j}}{\\sum_{i=1}^n \\sqrt{2b_i}} \\leq \\sum_{i=1}^n \\frac{(2a_i)}{\\sqrt{2b_i}}$$\n",
    "\n",
    "Step 6: Simplify\n",
    "$$\\frac{\\sum_{i=1}^n (2a_i)}{\\sum_{i=1}^n \\sqrt{2b_i}} \\leq \\sum_{i=1}^n \\frac{(2a_i)}{\\sqrt{2b_i}}\n",
    "$$"
   ]
  }
 ],
 "metadata": {
  "kernelspec": {
   "display_name": "base",
   "language": "python",
   "name": "python3"
  },
  "language_info": {
   "codemirror_mode": {
    "name": "ipython",
    "version": 3
   },
   "file_extension": ".py",
   "mimetype": "text/x-python",
   "name": "python",
   "nbconvert_exporter": "python",
   "pygments_lexer": "ipython3",
   "version": "3.11.7"
  }
 },
 "nbformat": 4,
 "nbformat_minor": 2
}
